Print exprs with correct (and minimal) parens

src/Util/PrintUtil.dfy
@@ -1,4 +1,11 @@
 module PrintUtil {
+  export
+    provides Indent, IndentAmount
+    provides CustomLiteralToString
+    reveals ExprFormatOption, BindingPower, Side, TieBreaker
+    provides ExprFormatOption.Space, ExprFormatOption.More
+    provides BindingPower.Init, BindingPower.EndlessOperator, BindingPower.SubexpressionPower
+    provides Parenthesis, ParenthesisWrap
 
   method Indent(indent: nat) {
     for i := 0 to indent {
@@ -6,7 +13,7 @@ module PrintUtil {
     }
   }
 
-  const IndentAmount := 2
+  const IndentAmount: nat := 2
 
   datatype ExprFormatOption = SingleLine | MultipleLines(indent: nat)
   {
@@ -24,5 +31,80 @@ module PrintUtil {
       case MultipleLines(indent) =>
         MultipleLines(indent + IndentAmount)
     }
+  }
+
+  function CustomLiteralToString(s: string, typeName: string): string {
+    "|" + s + ": " + typeName + "|"
+  }
+
+  // An operator (or keyword) appearing in an expression has a kind of "magnetism" on
+  // both sides. The magnetism says how much of a force the operator exerts to the left
+  // (on its leftmost subexpression) and to the right (on its rightmost subexpression).
+  //
+  //       expr    <--left force---  OPERATOR  ---right force-->    expr
+  //
+  // The context where the expression appears also exerts some force on both sides.
+  //
+  //       ---context force from left-->  expr  <--context force from right---
+  //
+  // If an operator exerts more force on its leftmost and rightmost arguments than
+  // the surrounding context, then it "wins" and no parentheses are needed when printing
+  // the expression in that context.
+  //
+  // 0 is the lowest force. It says that no claim is made on the expression in that direction.
+  //
+  // A left-associative operator has a slightly larger pull on its right argument.
+  // A right-associative operator has a slightly larger pull on its left argument.
+  //
+  // When the context and operator exert the same force on a subexpression, there are different
+  // ways of breaking the tie:
+  //     - operator wins
+  //     - context wins
+  //     - operator wins if both operator and context are of the same "family"
+  datatype BindingPower = BindingPower(left: nat, right: nat, tieBreaker: TieBreaker := OperatorWins)
+  {
+    static const Init := BindingPower(0, 0)
+    static const EndlessOperator := BindingPower(1000, 0)
+
+    predicate WinsOver(context: BindingPower) {
+      if tieBreaker.BreakTieInFavorOfOperator(context.tieBreaker) then
+        context.left <= left && context.right <= right
+      else
+        context.left < left && context.right < right
+    }
+
+    function SubexpressionPower(side: Side, context: BindingPower): BindingPower {
+      // adjust the context for parentheses that would have been added
+      var adjustedContext := if WinsOver(context) then context else Init;
+      match side
+      case Left => BindingPower(adjustedContext.left, left, tieBreaker)
+      case Right => BindingPower(right, adjustedContext.right, tieBreaker)
+    }
+  }
+
+  datatype Side = Left | Right
+
+  datatype TieBreaker = OperatorWins | ContextWins | SameFamilyWins(n: nat)
+  {
+    predicate BreakTieInFavorOfOperator(context: TieBreaker) {
+      || this == OperatorWins
+      || context == OperatorWins
+      || (this.SameFamilyWins? && this == context)
+    }
+  }
+
+  method Parenthesis(side: Side, opStrength: BindingPower, context: BindingPower) {
+    if !opStrength.WinsOver(context) {
+      match side
+      case Left => print "(";
+      case Right => print ")";
+    }
+  }
+
+  function ParenthesisWrap(opStrength: BindingPower, contextStrength: BindingPower, s: string): string {
+    if opStrength.WinsOver(contextStrength) then
+      s
+    else
+      "(" + s + ")"
   }
 }
